refactoring to remove duplicate specifications and other enhancements

thys/DataRefinementIBP/DataRefinement.thy
@@ -1,148 +1,158 @@
-header {*  Data Refinement of Diagrams *}
+header {* Data Refinement of Diagrams *}
 
 theory DataRefinement
 imports Diagram
 begin
 
 text{*
-Next definition introduces the concept of data refinement of $(\mathit{assert} \  q)\circ (\mathit{demonic}\ Q)$
-to $S$ using the data abstractions $R$ and $R'$.
+Next definition introduces the concept of data refinement of $S1$
+to $S2$ using the data abstractions $R$ and $R'$.
 *}
 
 definition
-  "DataRefinement p Q R R' S = (\<forall> s . \<Turnstile> {s' . s \<in> R s' \<and> s \<in> p} {| S |} (angelic R' (Q s)))"
+  DataRefinement :: "('a\<Colon>type \<Rightarrow> 'b\<Colon>type)
+     \<Rightarrow> ('b\<Colon>type \<Rightarrow> 'c\<Colon>ord) \<Rightarrow> ('a\<Colon>type \<Rightarrow> 'd\<Colon>type) 
+     \<Rightarrow> ('d\<Colon>type \<Rightarrow> 'c\<Colon>ord) \<Rightarrow> bool" where
+  "DataRefinement S1 R R' S2 = ((R o S1) \<le> (S2 o R'))"
 
 text{*
-The definition of the data refinement above is justified by the follwing two theorems.
-*}
-
-theorem datarefinement1:
-  "mono S \<Longrightarrow> ((angelic R) o (assert p) o (demonic Q) \<le> S) = (\<forall> s . \<Turnstile> {s' . R s' s \<and> p s} {| S |} (Q s))"
-  apply (simp add: le_fun_def assert_def angelic_def demonic_def Hoare_def le_bool_def)
-  apply safe
-  apply (simp_all add: Collect_def)
-  apply auto
-  apply (drule_tac x = "Q s" in spec)
-  apply (drule_tac x = "x" in spec)
-  apply auto
-  apply (unfold simp_eq_emptyset)
-  apply (drule_tac x = "s" in spec)
-  apply auto
-  apply (simp_all add: mem_def)
-  apply (simp add: mono_def)
-  by (metis rev_predicate1D)
-
-theorem datarefinement2:
-  "mono S \<Longrightarrow> ((angelic R) o (assert p) o (demonic Q) \<le> (S o (angelic R'))) = DataRefinement p Q R R' S"
-  apply (simp_all add: datarefinement1 mono_comp)
-  by (simp_all add: DataRefinement_def Hoare_def subset_eq mem_def)
-
-text{*
-If $\mathit{demonic}\ Q$ is correct with respect to $p$ and $q$, and $(\mathit{assert} \ p)\circ (\mathit{demonic}\  Q)$ 
-is data refined
-by $S$, then $S$ is correct with respect to $\mathit{angelic}\  R\  p$ and $\mathit{angelic} \ R' \ q$.
+If $\mathit{demonic}\ Q$ is correct with respect to $p$ and $q$, and 
+$(\mathit{assert} \ p)\circ (\mathit{demonic}\  Q)$ is data refined
+by $S$, then $S$ is correct with respect to $\mathit{angelic}\  R\  p$ and 
+$\mathit{angelic} \ R' \ q$.
 *}
 
 theorem data_refinement:
-  "mono S \<Longrightarrow> \<Turnstile> p {| demonic Q |} q \<Longrightarrow>  DataRefinement p Q R R' S \<Longrightarrow> 
-         \<Turnstile> (angelic R p) {| S |} (angelic R' q)"
-  apply (simp add: hoare_demonic DataRefinement_def angelic_def simp_eq_emptyset)
-  apply (simp add: Hoare_def less_fun_def)
-  apply safe
-  apply (drule_tac x = "{s . R' s \<sqinter> Q xa \<noteq> \<bottom>}" and y = "{s . R' s \<sqinter> q \<noteq> \<bottom>}" in monoD)
-  apply auto
-  apply (drule_tac x = xa in spec)
-  apply auto
-  apply (unfold subset_eq)
-  apply (unfold demonic_def)
-  apply (erule notE)
-  apply (rule antisym)
-  apply auto
-  apply (case_tac "R' xb \<sqinter> Q xa \<le> R' xb \<sqinter> q")
+  "mono R \<Longrightarrow> \<Turnstile> p {| S |} q \<Longrightarrow>  DataRefinement S R R' S' \<Longrightarrow> 
+         \<Turnstile> (R p) {| S' |} (R' q)"
+  apply (simp add:  DataRefinement_def Hoare_def le_fun_def)
+  apply (drule_tac x = q in spec)
+  apply (rule_tac y = "R (S q)" in order_trans)
+  apply (drule_tac x = p and y = "S q" in monoD)
+  by simp_all
+
+theorem data_refinement2:
+  "mono R \<Longrightarrow> \<Turnstile> p {| S |} q \<Longrightarrow>  DataRefinement ({.p.} o S) R R' S' \<Longrightarrow> 
+         \<Turnstile> (R p) {| S' |} (R' q)"
+  apply (simp add:  DataRefinement_def Hoare_def le_fun_def assert_def)
+  apply (drule_tac x = q in spec)
+  apply (subgoal_tac "p \<sqinter> S q = p")
   apply simp
-  apply (erule notE)
-  apply (rule_tac inf_greatest)
-  apply auto
-  apply (rule_tac y = "Q xa" in order_trans)
+  apply (rule antisym)
+  by simp_all
+
+theorem data_refinement_hoare:
+  "mono S \<Longrightarrow> mono D \<Longrightarrow> DataRefinement ({.p.} o [:Q:]) {:R:} D S = 
+         (\<forall> s . \<Turnstile> {s' . s \<in> R s' \<and> s \<in> p} {| S |} (D ((Q s)::'a::order)))"
+  apply (simp add: le_fun_def assert_def angelic_def demonic_def Hoare_def DataRefinement_def)
+  apply safe
+  apply (simp_all)
+  apply (drule_tac x = "Q s" in spec)
+  apply auto [1]
+  apply (drule_tac x = "xb" in spec)
+  apply simp
+  apply (simp add: less_eq_set_def le_fun_def)
+  apply (drule_tac x = xa in spec)
+  apply (simp_all add: mono_def)
   by auto
 
-
-theorem data_refinement_choice:
-  "DataRefinement p Q R R' S \<Longrightarrow> DataRefinement p Q R R' S' \<Longrightarrow> DataRefinement p Q R R' ( S \<sqinter> S') "
-  by (simp add: DataRefinement_def hoare_choice)
-
-theorem data_refinement_top [simp]:
-  "DataRefinement p Q R R' \<top>"
-  by (simp add: DataRefinement_def)
+theorem data_refinement_choice1:
+  "DataRefinement S1 D D' S2 \<Longrightarrow> DataRefinement S1 D D' S2' \<Longrightarrow> DataRefinement S1 D D' ( S2 \<sqinter> S2') "
+  by (simp add: DataRefinement_def hoare_choice le_fun_def inf_fun_def)
 
 
 theorem data_refinement_choice2:
-  "mono S \<Longrightarrow> mono S' \<Longrightarrow> DataRefinement p (Q::('a \<Rightarrow>'b::boolean_algebra)) R R' S \<Longrightarrow> DataRefinement p Q' R R' S' \<Longrightarrow> 
-     DataRefinement p (Q \<squnion> Q') R R' ( S \<sqinter> S')"
-  apply (simp add: DataRefinement_def sup_fun_def)
-  apply (simp add: angelic_disjunctive hoare_choice)
+  "mono D \<Longrightarrow> DataRefinement S1 D D' S2 \<Longrightarrow> DataRefinement S1' D D' S2' \<Longrightarrow> 
+     DataRefinement (S1 \<sqinter> S1') D D' (S2 \<sqinter> S2')"
+  apply (simp add: DataRefinement_def inf_fun_def le_fun_def)
   apply safe
-  apply (rule hoare_mono)
-  apply auto
-  apply (rule_tac S = S' and Q = "angelic R' (Q' s)" in  hoare_mono)
+  apply (rule_tac y = "D (S1 x)" in order_trans)
+  apply (drule_tac x = "S1 x \<sqinter> S1' x" and y = "S1 x" in monoD)
+  apply simp_all
+  apply (rule_tac y = "D (S1' x)" in order_trans)
+  apply (drule_tac x = "S1 x \<sqinter> S1' x" and y = "S1' x" in monoD)
+  by simp_all
+
+
+theorem data_refinement_top [simp]:
+  "DataRefinement S1 D D' \<top>"
+  by (simp add: DataRefinement_def le_fun_def top_fun_def)
+
+definition apply_fun::"('a\<Rightarrow>'b\<Rightarrow>'c)\<Rightarrow>('a\<Rightarrow>'b)\<Rightarrow>'a\<Rightarrow>'c" (infixl ".." 5) where
+  "(A .. B) = (\<lambda> x . (A x) (B x))"
+
+definition
+  "Disjunctive_fun R = (\<forall> i . (R i) \<in> Apply.Disjunctive)"
+
+lemma Disjunctive_Sup:
+  "Disjunctive_fun R \<Longrightarrow> (R .. (Sup X)) =  Sup {y . \<exists> x \<in> X . y = (R .. x)}"
+  apply (subst fun_eq_iff)
+  apply (simp add: Sup_fun_def apply_fun_def)
+  apply safe
+  apply (simp add: SUP_def apply_fun_def)
+  apply (subst (asm) Disjunctive_fun_def)
+  apply (drule_tac x = x in spec)
+  apply (simp add: Apply.Disjunctive_def)
+  apply (subgoal_tac "(R x ` (\<lambda>f. f x) ` X) =((\<lambda>f. f x) ` {y. \<exists>x\<in>X. y = (\<lambda>xa. R xa (x xa))})")
   by auto
 
-theorem (in DiagramTermination) dgr_data_refinement:
-  "dmono D \<Longrightarrow>
-   (\<forall> w i j . \<Turnstile> P w i  {| demonic (Q (i, j)) |} SUP_L_P P (pair w i) j) \<Longrightarrow>
-   (\<forall> w i j . DataRefinement (P w i) (Q (i,j)) (R i) (R j) (D (i, j))) \<Longrightarrow>
-   
-   \<Turnstile> (dangelic R (SUP P)) {| pt D |} ((dangelic R (SUP P)) \<sqinter> (-(grd (step D))))"
-
-  apply (simp add: dangelic_udisjunctive)
-  apply (rule hoare_diagram2)
-  apply (simp_all add: dangelic_def)
-  apply safe
-  apply (unfold dangelic_udisjunctive2)
-  apply (simp_all add: dangelic_def)
-  apply (rule data_refinement)
+lemma (in DiagramTermination) disjunctive_SUP_L_P:
+  "Disjunctive_fun R \<Longrightarrow> (R .. (SUP_L_P P (pair u i))) =  (SUP_L_P (\<lambda> w . (R .. (P w)))) (pair u i)"
+  apply (subst fun_eq_iff)
+  apply (simp add: SUP_L_P_def apply_fun_def SUP_def Disjunctive_fun_def Apply.Disjunctive_def, safe)
+  apply (subgoal_tac "(R x ` (\<lambda>v. P v x) ` {v. pair v x \<sqsubset> pair u i}) = 
+       ((\<lambda>v. R x (P v x)) ` {v. pair v x \<sqsubset> pair u i})")
   by auto
 
-theorem (in DiagramTermination) dgr_data_refinement1:
-  "dmono D \<Longrightarrow>
-   (\<forall> w i j . \<Turnstile> P w i  {| demonic (Q (i, j)) |} SUP_L_P P (pair w i) j) \<Longrightarrow>
-   (\<forall> i j . DataRefinement ((SUP P) i) (Q (i,j)) (R i) (R j) (D (i, j))) \<Longrightarrow>
-   
-   \<Turnstile> (dangelic R (SUP P)) {| pt D |} ((dangelic R (SUP P)) \<sqinter> (-(grd (step D))))"
+lemma apply_fun_range: "{y. \<exists>x. y = (R .. P x)} = range (\<lambda> x . R .. P x)"
+  by auto
 
-  apply (simp add: dangelic_udisjunctive)
+lemma [simp]: "Disjunctive_fun R \<Longrightarrow> mono ((R i)::'a::complete_lattice \<Rightarrow> 'b::complete_lattice)"
+  by (simp add: Disjunctive_fun_def)
+
+theorem (in DiagramTermination) dgr_data_refinement_1:
+  "dmono D' \<Longrightarrow> Disjunctive_fun R \<Longrightarrow>
+   (\<forall> w i j . \<Turnstile> P w i  {| D(i,j) |} SUP_L_P P (pair w i) j) \<Longrightarrow>
+   (\<forall> w i j . DataRefinement ((assert (P w i)) o (D (i,j))) (R i) (R j) (D' (i, j))) \<Longrightarrow>
+   
+   \<Turnstile> (R .. (Sup (range P))) {| pt D' |} ((R .. (Sup (range P))) \<sqinter> (-(grd (step D'))))"
+  apply (simp add: Disjunctive_Sup apply_fun_range)
   apply (rule hoare_diagram2)
-  apply (simp_all add: dangelic_def)
+  apply simp_all
   apply safe
-  apply (unfold dangelic_udisjunctive2)
-  apply (simp_all add: dangelic_def)
-  apply (rule data_refinement)
-  apply auto
-  apply (unfold DataRefinement_def)
-  apply safe
-  apply (rule_tac P = "{s' . s \<in> R i s' \<and> s \<in> SUP P i}" in hoare_pre)
-  apply auto
-  apply (simp add: SUP_def Sup_fun_def Sup_bool_def mem_def)
+  apply (simp add: disjunctive_SUP_L_P [THEN sym])
+  apply (simp add: apply_fun_def)
+  apply (rule_tac S = "D (i, j)" in data_refinement2)
   by auto
 
 definition
-  "DgrDataRefinement P T R D = (\<forall> i j . DataRefinement (P i) (T (i,j)) (R i) (R j) (D (i, j)))"
+  "DgrDataRefinement1 D R D' = (\<forall> i j . DataRefinement (D (i , j)) (R i) (R j) (D' (i, j)))"
 
+definition
+  "DgrDataRefinement2 P D R D' = (\<forall> i j . DataRefinement ({.P i.} o D (i , j)) (R i) (R j) (D' (i, j)))"
 
 theorem DataRefinement_mono:
-  "q \<le> p \<Longrightarrow> DataRefinement p Q R R' S \<Longrightarrow> DataRefinement q Q R R' S"
-  apply (simp add: DataRefinement_def)
-  apply auto
-  apply (drule_tac x = "s" in spec)
-  apply (rule hoare_pre)
-  by auto
-  
+  "T \<le> S \<Longrightarrow> mono R \<Longrightarrow> DataRefinement S R R' S' \<Longrightarrow> DataRefinement T R R' S' "
+  apply (simp add: DataRefinement_def mono_def)
+  apply (subst le_fun_def)
+  apply (simp add: le_fun_def)
+  apply safe
+  apply (rule_tac y = "R (S x)" in order_trans)
+  by simp_all
+
+definition
+  "mono_fun R = (\<forall> i . mono (R i))"
+
 theorem DgrDataRefinement_mono:
-  "Q \<le> P \<Longrightarrow> DgrDataRefinement P T R S \<Longrightarrow> DgrDataRefinement Q T R S"
-  apply (simp add: DgrDataRefinement_def)
+  "Q \<le> P \<Longrightarrow> mono_fun R \<Longrightarrow> DgrDataRefinement2 P D R D' \<Longrightarrow> DgrDataRefinement2 Q D R D'"
+  apply (simp add: DgrDataRefinement2_def)
   apply auto
-  apply (rule_tac p = "P i" and q = "Q i" in DataRefinement_mono)
-  by (simp_all add: le_fun_def mem_def le_bool_def)
+  apply (rule_tac S = "{.P i.} o D(i, j)" in DataRefinement_mono)
+  apply (simp_all add: le_fun_def assert_def)
+  apply safe
+  apply (rule_tac y = "Q i" in order_trans)
+  by (simp_all add: mono_fun_def)
+
 
 text{*
 Next theorem is the diagram version of the data refinement theorem. If the
@@ -152,22 +162,50 @@ if the diagram demonic choice $T$ terminates, then $D$ also terminates.
 *}
   
 
-theorem (in DiagramTermination) Diagram_DataRefinement:
-  "\<lbrakk> dmono D; \<turnstile> P {|dgr_demonic T|} Q; DgrDataRefinement P T R D \<rbrakk>  \<Longrightarrow>
-      \<turnstile> dangelic R P {| D |} ((dangelic R P) \<sqinter> (-(grd (step D))))" 
-
-  apply (unfold Hoare_dgr_def DgrDataRefinement_def dgr_demonic_def)
-  apply auto
-  apply (rule_tac x="\<lambda> w . dangelic R (X w)" in exI)
+theorem (in DiagramTermination) Diagram_DataRefinement1:
+  "dmono D \<Longrightarrow> Disjunctive_fun R \<Longrightarrow> \<turnstile> P {| D |} Q \<Longrightarrow> DgrDataRefinement1 D R D' \<Longrightarrow>
+      \<turnstile> (R .. P) {| D' |} ((R .. P) \<sqinter> (-(grd (step D'))))"
+  apply (unfold Hoare_dgr_def DgrDataRefinement1_def dgr_demonic_def)
   apply safe
-  apply (unfold dangelic_udisjunctive2)
-  apply (simp add: dangelic_def)
-  apply (rule_tac Q="T(i,j)" in data_refinement)
-  apply auto
-  apply (rule_tac p = "(SUP X i)" in DataRefinement_mono)
-  apply (simp add: SUP_def Sup_fun_def mem_def)
-  apply auto
-  apply (simp add: Sup_bool_def mem_def)
-  apply auto
-  by (simp_all add: dangelic_udisjunctive)
+  apply (rule_tac x="\<lambda> w . R .. (X w)" in exI)
+  apply safe
+  apply (unfold disjunctive_SUP_L_P [THEN sym])
+  apply (simp add: apply_fun_def)
+  apply (rule_tac S = "D (i,j)" and R = "R i" and R' = "R j" in data_refinement)
+  by (simp_all add: Disjunctive_Sup apply_fun_range)
+
+
+lemma comp_left_mono [simp]: "S \<le> S' \<Longrightarrow> S o T \<le> S' o T"
+  by (simp add: le_fun_def)
+
+lemma assert_pred_mono [simp]: "p \<le> q \<Longrightarrow> {.p.} \<le> {.q.}"
+  apply (simp add: le_fun_def assert_def)
+  apply safe
+  apply (rule_tac y = p in order_trans)
+  by simp_all
+
+theorem (in DiagramTermination) Diagram_DataRefinement2:
+  "dmono D \<Longrightarrow> Disjunctive_fun R \<Longrightarrow> \<turnstile> P {| D |} Q \<Longrightarrow> DgrDataRefinement2 P D R D' \<Longrightarrow>
+      \<turnstile> (R .. P) {| D' |} ((R .. P) \<sqinter> (-(grd (step D'))))"
+  apply (unfold Hoare_dgr_def DgrDataRefinement2_def dgr_demonic_def)
+  apply safe
+  apply (rule_tac x="\<lambda> w . R .. (X w)" in exI)
+  apply safe
+  apply (unfold disjunctive_SUP_L_P [THEN sym])
+  apply (simp add: apply_fun_def)
+  apply (rule_tac S = "D (i,j)" and R = "R i" and R' = "R j" in data_refinement2)
+  apply (simp_all add: Disjunctive_Sup)
+  apply (rule_tac S = "{.Sup (range X) i.} \<circ> D (i, j)" in DataRefinement_mono)
+  apply (rule comp_left_mono)
+  apply (rule assert_pred_mono)
+  apply (simp add: Sup_fun_def)
+  apply (rule SUP_upper)
+  by (simp_all add: apply_fun_range)
+
+lemma "(R'::'a::complete_lattice \<Rightarrow> 'b::complete_lattice) \<in> Apply.Disjunctive \<Longrightarrow>
+   DataRefinement S R R' S' \<Longrightarrow> R (- grd S) \<le> - grd S'"
+  apply (simp add: DataRefinement_def grd_def le_fun_def)
+  apply (drule_tac x = "\<bottom>" in spec)
+  by simp
+
 end
