thys/LatticeProperties/Complete_Lattice_Prop.thy
@@ -1,28 +1,21 @@
-header {* Complete Lattice Properties *}
+header {* Fixpoints and Complete Lattices *}
 
 (*
     Author: Viorel Preoteasa
 *)
 
 theory Complete_Lattice_Prop
-imports Main
+imports WellFoundedTransitive
 begin
 
 text{*
-This theory introduces some results about complete lattices. The
-main result is that a monotonic function mapping momotonic
-functions to monotonic functions has the least fixpoint monotonic.
+This theory introduces some results about fixpoints of functions on 
+complete lattices. The main result is that a monotonic function 
+mapping momotonic functions to monotonic functions has the least 
+fixpoint monotonic.
 *}
 
 context complete_lattice begin
-
-theorem Sup_bottom:
-  "(Sup X = bot) = (\<forall> x \<in> X . x = bot)"
-  by (rule Sup_bot_conv)
-
-theorem Inf_top:
-  "(Inf X = top) = (\<forall> x \<in> X . x = top)"
-  by (rule Inf_top_conv)
 
 lemma inf_Inf: assumes nonempty: "A \<noteq> {}"
    shows "inf x (Inf A) = Inf ((inf x) ` A)"
@@ -67,19 +60,26 @@ theorem lfp_mono [simp]:
   apply (rule SUP_upper)
   by auto
 
-
-class well_founded_transitive = ord +
-  assumes order_trans1: "x < y \<Longrightarrow> y < z \<Longrightarrow> x < z"
-  and less_eq_def: "x \<le> y <-> x = y \<or> x < y"
-  and less_induct1 [case_names less]: "(!!x . (!!y . y < x \<Longrightarrow> P y) \<Longrightarrow> P x) \<Longrightarrow> P a"
-
-
 context complete_lattice begin
 
 definition
-  "Sup_less x (w::'b::well_founded_transitive) = Sup {y . \<exists> v < w . y = x v}"
+  "Sup_less x (w::'b::well_founded) = Sup {y ::'a . \<exists> v < w . y = x v}"
+
+lemma Sup_less_upper:
+  "v < w \<Longrightarrow> P v \<le> Sup_less P w"
+  by (simp add: Sup_less_def, rule Sup_upper, blast)
+
+
+lemma Sup_less_least:
+  "(!! v . v < w \<Longrightarrow> P v \<le> Q) \<Longrightarrow> Sup_less P w \<le> Q"
+  by (simp add: Sup_less_def, rule Sup_least, blast)
 
 end
+
+lemma Sup_less_fun_eq:
+  "((Sup_less P w) i) = (Sup_less (\<lambda> v . P v i)) w"
+  apply (simp add: Sup_less_def Sup_fun_def SUP_def)
+  by (rule_tac f = Sup in arg_cong, auto)
 
 theorem fp_wf_induction:
   "f x  = x \<Longrightarrow> mono f \<Longrightarrow> (\<forall> w . (y w) \<le> f (Sup_less y w)) \<Longrightarrow> Sup (range y) \<le> x"
@@ -88,195 +88,6 @@ theorem fp_wf_induction:
   apply (rule less_induct1, simp_all)
   apply (rule_tac y = "f (Sup_less y xa)" in order_trans, simp)
   apply (drule_tac x = "Sup_less y xa" and y = "x" in monoD)
-  apply (simp add: Sup_less_def)
-  apply (rule Sup_least)
-  by auto
-
-locale conjunctive =
-  fixes inf_b :: "'b \<Rightarrow> 'b \<Rightarrow> 'b"
-  and inf_c :: "'c \<Rightarrow> 'c \<Rightarrow> 'c"
-  and times_abc :: "'a \<Rightarrow> 'b \<Rightarrow> 'c"
-begin
-
-definition
-  "conjunctive = {x . (\<forall> y z . times_abc x (inf_b y z) = inf_c (times_abc x y) (times_abc x z))}"
-
-lemma conjunctiveD: "x \<in> conjunctive \<Longrightarrow> times_abc x (inf_b y z) = inf_c (times_abc x y) (times_abc x z)"
-  by (simp add: conjunctive_def)
-
-end
-
-interpretation Apply: conjunctive "inf::'a::semilattice_inf \<Rightarrow> 'a \<Rightarrow> 'a"
-  "inf::'b::semilattice_inf \<Rightarrow> 'b \<Rightarrow> 'b" "\<lambda> f . f"
-  done
-
-interpretation Comp: conjunctive "inf::('a::lattice \<Rightarrow> 'a) \<Rightarrow> ('a \<Rightarrow> 'a) \<Rightarrow> ('a \<Rightarrow> 'a)" 
-  "inf::('a::lattice \<Rightarrow> 'a) \<Rightarrow> ('a \<Rightarrow> 'a) \<Rightarrow> ('a \<Rightarrow> 'a)" "(op o)"
-  done
-
-lemma "Apply.conjunctive = Comp.conjunctive"
-  apply (simp add: Apply.conjunctive_def Comp.conjunctive_def)
-  apply safe
-  apply (simp_all add: fun_eq_iff inf_fun_def)
-  apply (drule_tac x = "\<lambda> u . y" in spec)
-  apply (drule_tac x = "\<lambda> u . z" in spec)
-  by simp
-
-locale disjunctive =
-  fixes sup_b :: "'b \<Rightarrow> 'b \<Rightarrow> 'b"
-  and sup_c :: "'c \<Rightarrow> 'c \<Rightarrow> 'c"
-  and times_abc :: "'a \<Rightarrow> 'b \<Rightarrow> 'c"
-begin
-
-definition
-  "disjunctive = {x . (\<forall> y z . times_abc x (sup_b y z) = sup_c (times_abc x y) (times_abc x z))}"
-
-lemma disjunctiveD: "x \<in> disjunctive \<Longrightarrow> times_abc x (sup_b y z) = sup_c (times_abc x y) (times_abc x z)"
-  by (simp add: disjunctive_def)
-
-end
-
-interpretation Apply: disjunctive "sup::'a::semilattice_sup \<Rightarrow> 'a \<Rightarrow> 'a"
-  "sup::'b::semilattice_sup \<Rightarrow> 'b \<Rightarrow> 'b" "\<lambda> f . f"
-  done
-
-interpretation Comp: disjunctive "sup::('a::lattice \<Rightarrow> 'a) \<Rightarrow> ('a \<Rightarrow> 'a) \<Rightarrow> ('a \<Rightarrow> 'a)" 
-  "sup::('a::lattice \<Rightarrow> 'a) \<Rightarrow> ('a \<Rightarrow> 'a) \<Rightarrow> ('a \<Rightarrow> 'a)" "(op o)"
-  done
-
-lemma apply_comp_disjunctive: "Apply.disjunctive = Comp.disjunctive"
-  apply (simp add: Apply.disjunctive_def Comp.disjunctive_def)
-  apply safe
-  apply (simp_all add: fun_eq_iff sup_fun_def)
-  apply (drule_tac x = "\<lambda> u . y" in spec)
-  apply (drule_tac x = "\<lambda> u . z" in spec)
-  by simp
-
-locale Conjunctive =
-  fixes Inf_b :: "'b set \<Rightarrow> 'b"
-  and Inf_c :: "'c set \<Rightarrow> 'c"
-  and times_abc :: "'a \<Rightarrow> 'b \<Rightarrow> 'c"
-begin
-
-definition
-  "Conjunctive = {x . (\<forall> X . times_abc x (Inf_b X) = Inf_c ((times_abc x) ` X) )}"
-end
-
-interpretation Apply: Conjunctive Inf Inf "\<lambda> f . f"
-  done
-
-interpretation Comp: Conjunctive "Inf::(('a::complete_lattice \<Rightarrow> 'a) set) \<Rightarrow> ('a \<Rightarrow> 'a)" 
-  "Inf::(('a::complete_lattice \<Rightarrow> 'a) set) \<Rightarrow> ('a \<Rightarrow> 'a)" "(op o)"
-  done
-
-lemma fun_eq: "x = y \<Longrightarrow> f x = f y"
-  by simp
-
-lemma "Apply.Conjunctive = Comp.Conjunctive"
-  apply (simp add: Apply.Conjunctive_def Comp.Conjunctive_def)
-  apply safe
-  apply (simp add: fun_eq_iff  Inf_fun_def comp_def image_def)
-  apply (simp only: INF_def)
-  apply safe
-  apply (rule_tac f = Inf in fun_eq)
-  apply auto
-  apply (drule_tac x = "{x . \<exists> y \<in> X . x = (\<lambda> u . y)}" in spec)
-  apply (simp add: fun_eq_iff  Inf_fun_def comp_def image_def)
-  apply (drule_tac x = "bot" in spec)
-  apply (subgoal_tac "{y\<Colon>'a. \<exists>f . (\<exists>y \<in> X. \<forall>x::'a . f x = y) \<and> y = f bot} = X \<and> {y\<Colon>'a. \<exists>f. (\<exists>xa. (\<exists>y \<in> X. \<forall>x\<Colon>'a. xa x = y) \<and> (\<forall>xb\<Colon>'a. f xb = x (xa xb))) \<and> y = f bot} = {y\<Colon>'a. \<exists>xa\<Colon>'a\<in>X. y = x xa}")
-  apply (simp add: INF_def image_def, safe)
-  apply simp_all
-  apply auto[1]
-  apply auto [1]
-  apply (rule_tac x = "\<lambda> u . x xaa" in exI)
-  by auto
-
-
-locale Disjunctive =
-  fixes Sup_b :: "'b set \<Rightarrow> 'b"
-  and Sup_c :: "'c set \<Rightarrow> 'c"
-  and times_abc :: "'a \<Rightarrow> 'b \<Rightarrow> 'c"
-begin
-
-definition
-  "Disjunctive = {x . (\<forall> X . times_abc x (Sup_b X) = Sup_c ((times_abc x) ` X) )}"
-end
-
-interpretation Apply: Disjunctive Sup Sup "\<lambda> f . f"
-  done
-
-interpretation Comp: Disjunctive "Sup::(('a::complete_lattice \<Rightarrow> 'a) set) \<Rightarrow> ('a \<Rightarrow> 'a)" 
-  "Sup::(('a::complete_lattice \<Rightarrow> 'a) set) \<Rightarrow> ('a \<Rightarrow> 'a)" "(op o)"
-  done
-
-lemma "Apply.Disjunctive = Comp.Disjunctive"
-  apply (simp add: Apply.Disjunctive_def Comp.Disjunctive_def)
-  apply safe
-  apply (simp add: fun_eq_iff  Sup_fun_def comp_def image_def)
-  apply (simp only: SUP_def)
-  apply safe
-  apply (rule_tac f = Sup in fun_eq)
-  apply auto
-  apply (drule_tac x = "{x . \<exists> y \<in> X . x = (\<lambda> u . y)}" in spec)
-  apply (simp add: fun_eq_iff  Sup_fun_def comp_def image_def)
-  apply (drule_tac x = "bot" in spec)
-  apply (subgoal_tac "{y. \<exists>f::'a \<Rightarrow> 'a. (\<exists>y\<in>X. \<forall>x. f x = y) \<and> y = f bot} = X 
-    \<and> {y. \<exists>f::'a \<Rightarrow> 'a. (\<exists>xa. (\<exists>y\<in>X. \<forall>x. xa x = y) \<and> (\<forall>xb. f xb = x (xa xb))) \<and> y = f bot} = {y. \<exists>xa\<in>X. y = x xa}")
-  apply (simp add: SUP_def image_def, safe)
-  apply simp_all
-  apply auto[1]
-  apply auto [1]
-  apply (rule_tac x = "\<lambda> u . x xaa" in exI)
-  by auto
-
-
-lemma [simp]: "(F::'a::complete_lattice \<Rightarrow> 'b::complete_lattice) \<in> Apply.Conjunctive \<Longrightarrow> F \<in> Apply.conjunctive"
-  apply (simp add: Apply.Conjunctive_def Apply.conjunctive_def)
-  apply safe
-  apply (drule_tac x = "{y, z}" in spec)
-  by simp
-
-lemma [simp]: "F \<in> Apply.conjunctive \<Longrightarrow> mono F"
-  apply (simp add: Apply.conjunctive_def mono_def)
-  apply safe
-  apply (drule_tac x = "x" in spec)
-  apply (drule_tac x = "y" in spec)
-  apply (subgoal_tac "inf x y = x")
-  apply simp
-  apply (subgoal_tac "inf (F x) (F y) \<le> F y")
-  apply simp
-  apply (rule inf_le2)
-  apply (rule antisym)
-  by simp_all
-
-lemma [simp]: "(F::'a::complete_lattice \<Rightarrow> 'b::complete_lattice) \<in> Apply.Conjunctive \<Longrightarrow> F top = top"
-  apply (simp add: Apply.Conjunctive_def)
-  apply (drule_tac x="{}" in spec)
-  by (simp add: Inf_empty)
-
-lemma [simp]: "(F::'a::complete_lattice \<Rightarrow> 'b::complete_lattice) \<in> Apply.Disjunctive \<Longrightarrow> F \<in> Apply.disjunctive"
-  apply (simp add: Apply.Disjunctive_def Apply.disjunctive_def)
-  apply safe
-  apply (drule_tac x = "{y, z}" in spec)
-  by simp
-
-lemma [simp]: "F \<in> Apply.disjunctive \<Longrightarrow> mono F"
-  apply (simp add: Apply.disjunctive_def mono_def)
-  apply safe
-  apply (drule_tac x = "x" in spec)
-  apply (drule_tac x = "y" in spec)
-  apply (subgoal_tac "sup x y = y")
-  apply simp
-  apply (subgoal_tac "F x \<le> sup (F x) (F y)")
-  apply simp
-  apply (rule sup_ge1)
-  apply (rule antisym)
-  apply simp
-  by (rule sup_ge2)
-
-lemma [simp]: "(F::'a::complete_lattice \<Rightarrow> 'b::complete_lattice) \<in> Apply.Disjunctive \<Longrightarrow> F bot = bot"
-  apply (simp add: Apply.Disjunctive_def)
-  apply (drule_tac x="{}" in spec)
-  by (simp add: Sup_empty)
+  by (simp add: Sup_less_least, auto)
 
 end
