thys/LatticeProperties/Conj_Disj.thy
@@ -1,0 +1,205 @@
+header {* Conjunctive and Disjunctive Functions *}
+
+(*
+    Author: Viorel Preoteasa
+*)
+
+theory Conj_Disj
+imports Main
+begin
+
+text{*
+This theory introduces the definitions and some properties for 
+conjunctive, disjunctive, universally conjunctive, and universally 
+disjunctive functions.
+*}
+
+locale conjunctive =
+  fixes inf_b :: "'b \<Rightarrow> 'b \<Rightarrow> 'b"
+  and inf_c :: "'c \<Rightarrow> 'c \<Rightarrow> 'c"
+  and times_abc :: "'a \<Rightarrow> 'b \<Rightarrow> 'c"
+begin
+
+definition
+  "conjunctive = {x . (\<forall> y z . times_abc x (inf_b y z) = inf_c (times_abc x y) (times_abc x z))}"
+
+lemma conjunctiveD: "x \<in> conjunctive \<Longrightarrow> times_abc x (inf_b y z) = inf_c (times_abc x y) (times_abc x z)"
+  by (simp add: conjunctive_def)
+
+end
+
+interpretation Apply: conjunctive "inf::'a::semilattice_inf \<Rightarrow> 'a \<Rightarrow> 'a"
+  "inf::'b::semilattice_inf \<Rightarrow> 'b \<Rightarrow> 'b" "\<lambda> f . f"
+  done
+
+interpretation Comp: conjunctive "inf::('a::lattice \<Rightarrow> 'a) \<Rightarrow> ('a \<Rightarrow> 'a) \<Rightarrow> ('a \<Rightarrow> 'a)" 
+  "inf::('a::lattice \<Rightarrow> 'a) \<Rightarrow> ('a \<Rightarrow> 'a) \<Rightarrow> ('a \<Rightarrow> 'a)" "(op o)"
+  done
+
+lemma "Apply.conjunctive = Comp.conjunctive"
+  apply (simp add: Apply.conjunctive_def Comp.conjunctive_def)
+  apply safe
+  apply (simp_all add: fun_eq_iff inf_fun_def)
+  apply (drule_tac x = "\<lambda> u . y" in spec)
+  apply (drule_tac x = "\<lambda> u . z" in spec)
+  by simp
+
+locale disjunctive =
+  fixes sup_b :: "'b \<Rightarrow> 'b \<Rightarrow> 'b"
+  and sup_c :: "'c \<Rightarrow> 'c \<Rightarrow> 'c"
+  and times_abc :: "'a \<Rightarrow> 'b \<Rightarrow> 'c"
+begin
+
+definition
+  "disjunctive = {x . (\<forall> y z . times_abc x (sup_b y z) = sup_c (times_abc x y) (times_abc x z))}"
+
+lemma disjunctiveD: "x \<in> disjunctive \<Longrightarrow> times_abc x (sup_b y z) = sup_c (times_abc x y) (times_abc x z)"
+  by (simp add: disjunctive_def)
+
+end
+
+interpretation Apply: disjunctive "sup::'a::semilattice_sup \<Rightarrow> 'a \<Rightarrow> 'a"
+  "sup::'b::semilattice_sup \<Rightarrow> 'b \<Rightarrow> 'b" "\<lambda> f . f"
+  done
+
+interpretation Comp: disjunctive "sup::('a::lattice \<Rightarrow> 'a) \<Rightarrow> ('a \<Rightarrow> 'a) \<Rightarrow> ('a \<Rightarrow> 'a)" 
+  "sup::('a::lattice \<Rightarrow> 'a) \<Rightarrow> ('a \<Rightarrow> 'a) \<Rightarrow> ('a \<Rightarrow> 'a)" "(op o)"
+  done
+
+lemma apply_comp_disjunctive: "Apply.disjunctive = Comp.disjunctive"
+  apply (simp add: Apply.disjunctive_def Comp.disjunctive_def)
+  apply safe
+  apply (simp_all add: fun_eq_iff sup_fun_def)
+  apply (drule_tac x = "\<lambda> u . y" in spec)
+  apply (drule_tac x = "\<lambda> u . z" in spec)
+  by simp
+
+locale Conjunctive =
+  fixes Inf_b :: "'b set \<Rightarrow> 'b"
+  and Inf_c :: "'c set \<Rightarrow> 'c"
+  and times_abc :: "'a \<Rightarrow> 'b \<Rightarrow> 'c"
+begin
+
+definition
+  "Conjunctive = {x . (\<forall> X . times_abc x (Inf_b X) = Inf_c ((times_abc x) ` X) )}"
+end
+
+interpretation Apply: Conjunctive Inf Inf "\<lambda> f . f"
+  done
+
+interpretation Comp: Conjunctive "Inf::(('a::complete_lattice \<Rightarrow> 'a) set) \<Rightarrow> ('a \<Rightarrow> 'a)" 
+  "Inf::(('a::complete_lattice \<Rightarrow> 'a) set) \<Rightarrow> ('a \<Rightarrow> 'a)" "(op o)"
+  done
+
+lemma fun_eq: "x = y \<Longrightarrow> f x = f y"
+  by simp
+
+lemma "Apply.Conjunctive = Comp.Conjunctive"
+  apply (simp add: Apply.Conjunctive_def Comp.Conjunctive_def)
+  apply safe
+  apply (simp add: fun_eq_iff  Inf_fun_def comp_def image_def)
+  apply (simp only: INF_def)
+  apply safe
+  apply (rule_tac f = Inf in fun_eq)
+  apply auto
+  apply (drule_tac x = "{x . \<exists> y \<in> X . x = (\<lambda> u . y)}" in spec)
+  apply (simp add: fun_eq_iff  Inf_fun_def comp_def image_def)
+  apply (drule_tac x = "bot" in spec)
+  apply (subgoal_tac "{y\<Colon>'a. \<exists>f . (\<exists>y \<in> X. \<forall>x::'a . f x = y) \<and> y = f bot} = X \<and> 
+      {y\<Colon>'a. \<exists>f. (\<exists>xa. (\<exists>y \<in> X. \<forall>x\<Colon>'a. xa x = y) \<and> 
+      (\<forall>xb\<Colon>'a. f xb = x (xa xb))) \<and> y = f bot} = {y\<Colon>'a. \<exists>xa\<Colon>'a\<in>X. y = x xa}")
+  apply (simp add: INF_def image_def, safe)
+  apply simp_all
+  apply auto[1]
+  apply auto [1]
+  apply (rule_tac x = "\<lambda> u . x xaa" in exI)
+  by auto
+
+locale Disjunctive =
+  fixes Sup_b :: "'b set \<Rightarrow> 'b"
+  and Sup_c :: "'c set \<Rightarrow> 'c"
+  and times_abc :: "'a \<Rightarrow> 'b \<Rightarrow> 'c"
+begin
+
+definition
+  "Disjunctive = {x . (\<forall> X . times_abc x (Sup_b X) = Sup_c ((times_abc x) ` X) )}"
+end
+
+interpretation Apply: Disjunctive Sup Sup "\<lambda> f . f"
+  done
+
+interpretation Comp: Disjunctive "Sup::(('a::complete_lattice \<Rightarrow> 'a) set) \<Rightarrow> ('a \<Rightarrow> 'a)" 
+  "Sup::(('a::complete_lattice \<Rightarrow> 'a) set) \<Rightarrow> ('a \<Rightarrow> 'a)" "(op o)"
+  done
+
+lemma apply_comp_Disjunctive: "Apply.Disjunctive = Comp.Disjunctive"
+  apply (simp add: Apply.Disjunctive_def Comp.Disjunctive_def)
+  apply safe
+  apply (simp add: fun_eq_iff  Sup_fun_def comp_def image_def)
+  apply (simp only: SUP_def)
+  apply safe
+  apply (rule_tac f = Sup in fun_eq)
+  apply auto
+  apply (drule_tac x = "{x . \<exists> y \<in> X . x = (\<lambda> u . y)}" in spec)
+  apply (simp add: fun_eq_iff  Sup_fun_def comp_def image_def)
+  apply (drule_tac x = "bot" in spec)
+  apply (subgoal_tac "{y. \<exists>f::'a \<Rightarrow> 'a. (\<exists>y\<in>X. \<forall>x. f x = y) \<and> y = f bot} = X 
+    \<and> {y. \<exists>f::'a \<Rightarrow> 'a. (\<exists>xa. (\<exists>y\<in>X. \<forall>x. xa x = y) \<and> (\<forall>xb. f xb = x (xa xb))) \<and> y = f bot} = {y. \<exists>xa\<in>X. y = x xa}")
+  apply (simp add: SUP_def image_def, safe)
+  apply simp_all
+  apply auto[1]
+  apply auto [1]
+  apply (rule_tac x = "\<lambda> u . x xaa" in exI)
+  by auto
+
+
+lemma [simp]: "(F::'a::complete_lattice \<Rightarrow> 'b::complete_lattice) \<in> Apply.Conjunctive \<Longrightarrow> F \<in> Apply.conjunctive"
+  apply (simp add: Apply.Conjunctive_def Apply.conjunctive_def)
+  apply safe
+  apply (drule_tac x = "{y, z}" in spec)
+  by simp
+
+lemma [simp]: "F \<in> Apply.conjunctive \<Longrightarrow> mono F"
+  apply (simp add: Apply.conjunctive_def mono_def)
+  apply safe
+  apply (drule_tac x = "x" in spec)
+  apply (drule_tac x = "y" in spec)
+  apply (subgoal_tac "inf x y = x")
+  apply simp
+  apply (subgoal_tac "inf (F x) (F y) \<le> F y")
+  apply simp
+  apply (rule inf_le2)
+  apply (rule antisym)
+  by simp_all
+
+lemma [simp]: "(F::'a::complete_lattice \<Rightarrow> 'b::complete_lattice) \<in> Apply.Conjunctive \<Longrightarrow> F top = top"
+  apply (simp add: Apply.Conjunctive_def)
+  apply (drule_tac x="{}" in spec)
+  by simp
+
+lemma [simp]: "(F::'a::complete_lattice \<Rightarrow> 'b::complete_lattice) \<in> Apply.Disjunctive \<Longrightarrow> F \<in> Apply.disjunctive"
+  apply (simp add: Apply.Disjunctive_def Apply.disjunctive_def)
+  apply safe
+  apply (drule_tac x = "{y, z}" in spec)
+  by simp
+
+lemma [simp]: "F \<in> Apply.disjunctive \<Longrightarrow> mono F"
+  apply (simp add: Apply.disjunctive_def mono_def)
+  apply safe
+  apply (drule_tac x = "x" in spec)
+  apply (drule_tac x = "y" in spec)
+  apply (subgoal_tac "sup x y = y")
+  apply simp
+  apply (subgoal_tac "F x \<le> sup (F x) (F y)")
+  apply simp
+  apply (rule sup_ge1)
+  apply (rule antisym)
+  apply simp
+  by (rule sup_ge2)
+
+lemma [simp]: "(F::'a::complete_lattice \<Rightarrow> 'b::complete_lattice) \<in> Apply.Disjunctive \<Longrightarrow> F bot = bot"
+  apply (simp add: Apply.Disjunctive_def)
+  apply (drule_tac x="{}" in spec)
+  by simp
+
+end
